1. VST is updated. 2. VST version of instance of MSL and sMSL is added.

veric_ext/SeparationLogic.v
@@ -2,8 +2,78 @@ Require Import VST.veric.SeparationLogic.
 Require Import RamifyCoq.msl_ext.abs_addr.
 Require Import RamifyCoq.msl_ext.seplog.
 Require Import RamifyCoq.msl_ext.alg_seplog.
+Require Import RamifyCoq.veric_ext.seplog.
 
 Instance PSLveric: PreciseSepLog mpred := algPreciseSepLog compcert_rmaps.RML.R.rmap.
 Instance OSLveric: OverlapSepLog mpred := algOverlapSepLog compcert_rmaps.RML.R.rmap.
 Instance DSLveric: DisjointedSepLog mpred := algDisjointedSepLog compcert_rmaps.RML.R.rmap.
 
+Module Mapsto.
+Section Mapsto.
+
+Definition adr_conflict (a1 a2 : val * type) : bool :=
+  match a1, a2 with
+  | (p1, t1), (p2, t2) => 
+    if (pointer_range_overlap_dec p1 (BV_sizeof t1) p2 (BV_sizeof t2)) then true else false
+  end.
+
+Instance AbsAddr_veric : AbsAddr.
+  apply (mkAbsAddr (val * type) val adr_conflict); intros; unfold adr_conflict in *; destruct p1, p2.
+  + destruct (pointer_range_overlap_dec v (BV_sizeof t) v0 (BV_sizeof t0)); subst;
+    destruct (pointer_range_overlap_dec v0 (BV_sizeof t0) v (BV_sizeof t)); subst; auto;
+    pose proof pointer_range_overlap_comm v (BV_sizeof t) v0 (BV_sizeof t0);
+    tauto.
+  + destruct (pointer_range_overlap_dec v (BV_sizeof t) v0 (BV_sizeof t0)); auto.
+    destruct (pointer_range_overlap_isptr _ _ _ _ p).
+    destruct (zlt 0 (BV_sizeof t)).
+    - assert (pointer_range_overlap v (BV_sizeof t) v (BV_sizeof t))
+        by (apply pointer_range_overlap_refl; auto; omega).
+      destruct (pointer_range_overlap_dec v (BV_sizeof t) v (BV_sizeof t)); [congruence | tauto].
+    - apply pointer_range_overlap_non_zero in p.
+      omega.
+Defined.
+
+Instance MSLveric sh: MapstoSepLog AbsAddr_veric (fun pt v => let (p, t) := pt in mapsto sh t p v).
+Proof.
+  apply mkMapstoSepLog.
+  intros [p t].
+  apply exp_mapsto_precise.
+Defined.
+
+Instance sMSLveric sh: StaticMapstoSepLog AbsAddr_veric (fun pt v => let (p, t) := pt in mapsto sh t p v).
+Proof.
+  apply mkStaticMapstoSepLog.
+  + intros [p t] v ?.
+    unfold addr_empty in H; simpl in H.
+    destruct (pointer_range_overlap_dec p (BV_sizeof t) p (BV_sizeof t)); [congruence |].
+    unfold mapsto.
+    destruct (access_mode t) eqn:?H; try apply FF_left.
+    destruct (type_is_volatile t), p; try apply FF_left.
+    assert (pointer_range_overlap (Vptr b i) (BV_sizeof t) (Vptr b i) (BV_sizeof t)); [| tauto].
+    apply pointer_range_overlap_refl.
+    - simpl; tauto.
+    - eapply BV_sizeof_pos; eauto.
+    - eapply BV_sizeof_pos; eauto.
+  + intros [p1 t1] [p2 t2] v1 v2 ?.
+    apply mapsto_conflict with (PTree.empty _).
+    apply pointer_range_overlap_BV_sizeof.
+    simpl in H.
+    destruct (pointer_range_overlap_dec p1 (BV_sizeof t1) p2 (BV_sizeof t2)); [auto | congruence].
+  + intros [p1 t1] [p2 t2] ?.
+    simpl in H.
+    destruct (pointer_range_overlap_dec p1 (BV_sizeof t1) p2 (BV_sizeof t2)); [congruence |].
+    destruct (pointer_range_overlap_dec p1 (sizeof (PTree.empty _) t1) p2 (sizeof (PTree.empty _) t2)).
+    - apply pointer_range_overlap_sizeof with (sh := sh) in p.
+      destruct p as [? | [? | ?]].
+      * tauto.
+      * eapply disj_derives; [exact H0 | apply derives_refl |].
+        pose proof log_normalize.FF_disj.
+        simpl in H1; apply H1.
+      * eapply disj_derives; [apply derives_refl | exact H0 |].
+        pose proof log_normalize.disj_FF.
+        simpl in H1; apply H1.
+    - apply disj_mapsto_ with (PTree.empty _); auto.
+Defined.
+
+End Mapsto.
+End Mapsto.
